An automated theorem prover for first-order logic. For any provable formula, this program is guaranteed to find the proof (eventually). However, as a consequence of the negative answer to Hilbert's *Entscheidungsproblem*, there are some unprovable formulae that will cause this program to loop forever.

Some notes:

* The proof steps are shown as [sequents](http://en.wikipedia.org/wiki/Sequent).
* The actual theorem prover is in `prover.py`. The command-line interface (including the parser) is in `main.py`. `language.py` contains boilerplate classes used to represent logical formulae.
* The system will not accept a lemma unless it can be proven. An axiom is admitted without proof.
* This is only a pedagogical tool. It is too slow to be used for anything practical.

To get started, run `main.py`:

    $ ./main.py

    Terms:

      x               (variable)
      f(term, ...)    (function)

    Formulae:

      P(term)        (predicate)
      not P          (complement)
      P or Q         (disjunction)
      P and Q        (conjunction)
      P implies Q    (implication)
      forall x. P    (universal quantification)
      exists x. P    (existential quantification)

    Enter formulae at the prompt. The following commands are also available for manipulating axioms:

      axioms              (list axioms)
      lemmas              (list lemmas)
      axiom <formula>     (add an axiom)
      lemma <formula>     (prove and add a lemma)
      remove <formula>    (remove an axiom or lemma)
      reset               (remove all axioms and lemmas)

    >

Example session:

    > P or not P
    0. ⊢ (P ∨ ¬P)
    1. ⊢ P, ¬P
    2. P ⊢ P
    Formula proven: (P ∨ ¬P).

    > P and not P
    0. ⊢ (P ∧ ¬P)
    1. ⊢ P
    Formula unprovable: (P ∧ ¬P).

    > forall x. P(x) implies (Q(x) implies P(x))
    0. ⊢ (∀x. (P(x) → (Q(x) → P(x))))
    1. ⊢ (P(v1) → (Q(v1) → P(v1)))
    2. P(v1) ⊢ (Q(v1) → P(v1))
    3. Q(v1), P(v1) ⊢ P(v1)
    Formula proven: (∀x. (P(x) → (Q(x) → P(x)))).

    > exists x. (P(x) implies forall y. P(y))
    0. ⊢ (∃x. (P(x) → (∀y. P(y))))
    1. ⊢ (P(t1) → (∀y. P(y))), (∃x. (P(x) → (∀y. P(y))))
    2. P(t1) ⊢ (∀y. P(y)), (∃x. (P(x) → (∀y. P(y))))
    3. P(t1) ⊢ (∀y. P(y)), (P(t2) → (∀y. P(y))), (∃x. (P(x) → (∀y. P(y))))
    4. P(t1) ⊢ (P(t2) → (∀y. P(y))), (∃x. (P(x) → (∀y. P(y)))), P(v1)
    5. P(t1), P(t2) ⊢ (∀y. P(y)), (∃x. (P(x) → (∀y. P(y)))), P(v1)
    6. P(t1), P(t2) ⊢ (∀y. P(y)), (P(t3) → (∀y. P(y))), (∃x. (P(x) → (∀y. P(y)))), P(v1)
    7. P(t1), P(t2) ⊢ (P(t3) → (∀y. P(y))), P(v2), (∃x. (P(x) → (∀y. P(y)))), P(v1)
    8. P(t3), P(t1), P(t2) ⊢ (∀y. P(y)), P(v2), (∃x. (P(x) → (∀y. P(y)))), P(v1)
      t3 = v1
    Formula proven: (∃x. (P(x) → (∀y. P(y)))).

    > axiom forall x. Equals(x, x)
    Axiom added: (∀x. Equals(x, x)).

    > axioms
    (∀x. Equals(x, x))

    > lemma Equals(a, a)
    0. (∀x. Equals(x, x)) ⊢ Equals(a, a)
    1. Equals(t1, t1), (∀x. Equals(x, x)) ⊢ Equals(a, a)
      t1 = a
    Lemma proven: Equals(a, a).

    > lemmas
    Equals(a, a)

    > remove forall x. Equals(x, x)
    Axiom removed: (∀x. Equals(x, x)).
    This lemma was proven using that axiom and was also removed:
      Equals(a, a)
